isabelle/Foundations.thy
@@ -7,9 +7,10 @@ begin
 chapter \<open>Foundations\<close>
 text \<open>\label{chap:foundations}\<close>
 
-text \<open>In this section, the concepts that are relevant for the main part of this thesis will be introduced in text, as well as formalised in Isabelle. The formalisations of \cref{sec:LTS,sec:strong_bisimilarity} are based on those done by Benjamin Bisping in \cite{bisping2018computing}; the code is available on GitHub.%
+text \<open>In this chapter, the concepts that are relevant for the main part of this thesis will be introduced in text, as well as formalised in Isabelle. The formalisations of \cref{sec:LTS,sec:strong_bisimilarity} are based on those done by Benjamin Bisping in \cite{bisping2019computing} (the code is available on GitHub%
 \footnote{see \code{\href{https://coupledsim.bbisping.de/code/}%
-{coupledsim.bbisping.de/code/}}}
+{coupledsim.bbisping.de/code/}}}%
+).
 All other formalisations were done as part of this thesis.\<close>
 
 (*<*)
