isabelle/HM_Logic_infinitary.thy
@@ -8,9 +8,11 @@ begin
 chapter \<open>Infinitary Hennessy-Milner Logic\<close>
 text \<open>\label{chap:HML_infinitary}\<close>
 
-text \<open>We will show that a modal characterisation of strong bisimilarity is possible without any assumptions about the cardinality of derivative sets \<open>Der(p, \<alpha>)\<close>, using infinitary HML (with conjunction of arbitrary cardinality). Instead of formalising formulas under a conjunction as a countable set,%
-\footnote{Note that it is not possible to define a dataype with a constructor depending on a set of the type itself, i.e.\@ \<open>HML_conj \<open>('a)HML_formula set\<close>\<close> would not yield a valid data type. Dunno y tho.}
-we use an index set of arbitrary type \<open>I :: 'x set\<close> and a mapping \<open>F :: 'x \<Rightarrow> ('a, 'x)HML_formula\<close> so that each element of \<open>I\<close> is mapped to a formula. This closely resembles the semantics of $\bigwedge_{i \in I} \varphi_i$. Since the mapping is total, we cannot use the empty conjunction as a base for the type. Instead of using partial mappings \<open>F :: 'x \<Rightarrow> ('a, 'x)HML_formula option\<close>, I included a constructor \<open>HML_true\<close> and implicitly assume that \<open>F\<close> maps to \<open>HML_true\<close> for all objects of type \<open>'x\<close> that are not elements of \<open>I\<close>.\<close>
+text \<open>We will show that a modal characterisation of strong bisimilarity is possible without any assumptions about the cardinality of derivative sets \<open>Der(p, \<alpha>)\<close>, using infinitary HML (with conjunction of arbitrary cardinality). 
+
+Instead of formalising formulas under a conjunction as a countable set,%
+\footnote{Note that it is impossible to define a type with a constructor depending on a set of the type itself, i.e.\@ \<open>HML_conj \<open>('a)HML_formula set\<close>\<close> would not yield a valid type.}
+we use an index set of arbitrary type \<open>I :: 'x set\<close> and a mapping \linebreak \<open>F :: 'x \<Rightarrow> ('a, 'x)HML_formula\<close> so that each element of \<open>I\<close> is mapped to a formula. This closely resembles the semantics of $\bigwedge_{i \in I} \varphi_i$. Instead of using partial mappings \<open>F :: 'x \<Rightarrow> ('a, 'x)HML_formula option\<close>, I included a constructor \<open>HML_true\<close> and implicitly assume that \<open>F\<close> maps to \<open>HML_true\<close> for all objects of type \<open>'x\<close> that are not elements of \<open>I\<close>.\<close>
 
 datatype ('a, 'x)HML_formula =
   HML_true 
@@ -21,9 +23,14 @@ datatype ('a, 'x)HML_formula =
 
 subsubsection \<open>Satisfaction Relation\<close>
 
-text \<open>Data types cannot be used with arbitrary parameter types \<open>'x\<close> in concrete contexts; so when using our data type in the \<open>context lts\<close>, we use the type of processes \<open>'s\<close> as the type for conjunction index sets. Since this suffices to proof the modal characterisation, we can conclude that it suffices for the cardinality of conjunction to be equal to the cardinality of the set of processes $\Proc$. As we can deduce from the part of the proof where formula conjunction is used, a weaker requirement would be to allow for conjunction of cardinality equal to $\displaystyle\max_{\substack{p\in\Proc \\ \alpha\in\Act}} |\text{Der}(p, \alpha)|$.
+text \<open>Data types cannot be used with arbitrary parameter types \<open>'x\<close> in concrete contexts; so when using our data type in the \<open>context lts\<close>, we use the type of processes \<open>'s\<close> as the type for conjunction index sets. 
 
-The remainder of this section follows the same structure as \cref{sec:HML}. The explanations from there mostly apply here as well.\<close>
+\pagebreak
+Since this suffices to proof the modal characterisation, we can conclude that it suffices for the cardinality of conjunction to be equal to the cardinality of the set of processes $\Proc$. As we can deduce from the part of the proof where formula conjunction is used, a weaker requirement would be to allow for conjunction of cardinality equal to $\displaystyle\max_{\substack{p\in\Proc \\ \alpha\in\Act}} |\text{Der}(p, \alpha)|$.\<close>
+
+subsection \<open>Isabelle\<close>
+
+text \<open>The formalisation of this appendix follows the same structure as that in \cref{sec:HML}. The explanations from there mostly apply here as well.\<close>
 
 context lts begin
 
@@ -61,7 +68,7 @@ qed
 termination\<^marker>\<open>tag (proof) visible\<close> satisfies using HML_wf_rel_is_wf 
   by (standard, (simp add: HML_wf_rel.intros)+)
 
-
+text \<open>\newpage\<close>
 subsubsection \<open>Modal Characterisation of Strong Bisimilarity\<close>
 
 definition HML_equivalent :: \<open>'s \<Rightarrow> 's \<Rightarrow> bool\<close>
@@ -109,7 +116,7 @@ next
     by (meson satisfies.simps(4) strongly_bisimilar_step(1))
 qed
 
-
+text \<open>\newpage\<close>
 lemma\<^marker>\<open>tag (proof) visible\<close> HML_equivalence_is_SB:
   shows \<open>SB HML_equivalent\<close>
 proof -
@@ -127,17 +134,14 @@ proof -
     
     from "exists_\<phi>\<^bsub>q'\<^esub>" have \<open>p' \<Turnstile> ?\<phi>\<close>
       by (smt (z3) satisfies.simps(2) someI_ex)
-    hence \<open>p \<Turnstile> HML_poss \<alpha> ?\<phi>\<close> using \<open>p \<longmapsto>\<alpha> p'\<close>
-      by auto
+    hence \<open>p \<Turnstile> HML_poss \<alpha> ?\<phi>\<close> using \<open>p \<longmapsto>\<alpha> p'\<close> by auto
 
     from "exists_\<phi>\<^bsub>q'\<^esub>" have \<open>\<forall>q' \<in> Der(q, \<alpha>). \<not> q' \<Turnstile> ?\<phi>\<close>
       by (smt (z3) satisfies.simps(2) someI_ex)
-    hence \<open>\<not> q \<Turnstile> HML_poss \<alpha> ?\<phi>\<close>
-      by simp
+    hence \<open>\<not> q \<Turnstile> HML_poss \<alpha> ?\<phi>\<close> by simp
   
     from \<open>p \<Turnstile> HML_poss \<alpha> ?\<phi>\<close> \<open>\<not> q \<Turnstile> HML_poss \<alpha> ?\<phi>\<close> have False 
-      using \<open>HML_equivalent p q\<close> 
-      unfolding HML_equivalent_def by blast
+      using \<open>HML_equivalent p q\<close> HML_equivalent_def by blast
   }
 
   thus \<open>SB HML_equivalent\<close> unfolding SB_def 
