isabelle/Strong_Bisimilarity.thy
@@ -12,20 +12,27 @@ text \<open>As discussed in the previous section, LTSs can describe the behaviou
 Bisimilarity (or \emph{strong bisimilarity}, to be precise) is the \enquote{\emph{finest extensional behavioural equivalence} \textelp{} on processes} @{cite introBC}, an extensional property being one that treats the system in question as a black box, i.e.\@ the specific state space of the system remains hidden and performed transitions are only observable in terms of their action-label. This distinguishes bisimilarity from stronger graph equivalences like \emph{graph isomorphism}, where the (intensional) identity of processes (graph nodes) is relevant @{cite advBC_origins}.
 
 \example{%
-The processes $p$ and $q$ are strongly bisimilar, as both can always perform an a-transition and no transitions afterwards. There is no isomorphism between the left and right subgraphs, as they have a different number of nodes.
+The processes $p$ and $q$ are strongly bisimilar (written $p \leftrightarrow q$, following @{cite rbs}), as both can always perform exactly two a-transitions and no further transitions afterwards. There is no isomorphism between the left and right subgraphs, as they have a different number of nodes.
 
 \lts{
     \node[state]    (p0)                            {$p$};
     \node[state]    (p1) [below left of=p0]         {$p_1$};
-    \node[state]    (p2) [below right of=p0]        {$p_2$};
+    \node[state]    (p2) [below of=p1]              {$p_2$};
+    \node[state]    (p3) [below right of=p0]        {$p_3$};
+    \node[state]    (p4) [below of=p3]              {$p_4$};
     \node[state]    (q0) [right of=p0,xshift=2cm]   {$q$};
     \node[state]    (q1) [below of=q0]              {$q_1$};
+    \node[state]    (q2) [below of=q1]              {$q_2$};
     
     \path   (p0) edge node[above left]  {$a$}   (p1)
-                 edge node              {$a$}   (p2)
-            (q0) edge node              {$a$}   (q1);
+                 edge node              {$a$}   (p3)
+            (p1) edge node[left]        {$a$}   (p2)
+            (p3) edge node[left]        {$a$}   (p4)
+            (q0) edge node              {$a$}   (q1)
+            (q1) edge node              {$a$}   (q2);
 }}
 
+\pagebreak
 It is important to note that not only transitions that are performable, but also those that are not, are relevant.
 
 \example{%
@@ -47,10 +54,9 @@ The processes $p$ and $q$ are not strongly bisimilar, as $p$ can perform an $a$-
             (q1) edge node              {$a$}   (q2);
 }}
 
-Strong bisimilarity is the \emph{finest} extensional behavioural equivalence, because all actions of an LTS are thought of as observable and blockable. An example of a coarser equivalence is \emph{weak bisimilarity}, which treats the aforementioned hidden action $\tau$ as unobservable and unblockable. However, weak bisimilarity is of no further relevance for this thesis and the interested reader is referred to @{cite \<open>Chapter 3.4\<close> resyst}.
+Strong bisimilarity is the \emph{finest} extensional behavioural equivalence, because all actions are thought of as observable. An example of a coarser equivalence is \emph{weak bisimilarity}, which treats the aforementioned hidden action $\tau$ as unobservable. However, weak bisimilarity is of no further relevance for this thesis and the interested reader is referred to @{cite \<open>Chapter 3.4\<close> resyst}.
 
-This notion of strong bisimilarity can be formalised through \emph{strong bisimulation} (SB) relations, introduced originally by David Park in @{cite park81}. A binary relation $\mathcal{R}$ over the set of processes $\Proc$ is an SB iff for all $(p,q) \in \mathcal{R}$:
-
+The notion of strong bisimilarity can be formalised through \emph{strong bisimulation} (SB) relations, introduced originally by David Park in @{cite park81}. A binary relation $\mathcal{R}$ over the set of processes $\Proc$ is an SB iff for all $(p,q) \in \mathcal{R}$:
 \begin{align*}
 &\forall p' \in \Proc,\; \alpha \in \Act .\; p \xrightarrow{\alpha} p' \longrightarrow
 \exists q' \in \Proc .\; q \xrightarrow{\alpha} q' \wedge (p',q') \in \mathcal{R}, \text{ and}\\
@@ -71,7 +77,8 @@ definition SB :: \<open>('s \<Rightarrow> 's \<Rightarrow> bool) \<Rightarrow> b
     (\<forall> p' \<alpha>. p \<longmapsto>\<alpha> p' \<longrightarrow> (\<exists> q'. (q \<longmapsto>\<alpha> q') \<and> R p' q')) \<and>
     (\<forall> q' \<alpha>. q \<longmapsto>\<alpha> q' \<longrightarrow> (\<exists> p'. (p \<longmapsto>\<alpha> p') \<and> R p' q'))\<close>
 
-text \<open>Two processes $p$ and $q$ are then strongly bisimilar (written $p \leftrightarrow q$, following @{cite rbs}) iff there is an SB that contains the pair $(p, q)$.\<close>
+text \<open>\pagebreak
+Two processes $p$ and $q$ are then strongly bisimilar iff there is an SB that contains the pair $(p, q)$.\<close>
 
 definition strongly_bisimilar :: \<open>'s \<Rightarrow> 's \<Rightarrow> bool\<close> 
   (\<open>_ \<leftrightarrow> _\<close> [70, 70] 70)
